examples/map/MapIAproof.v
@@ -4,24 +4,22 @@ Require Import MapHeader MapA MapM MapI ModSim MapIMproof MapMAproof MemA wsim.
 
 Module MapIA. Section MapIA.
   Context `{!invG α Σ Γ, !subG Γ Σ, !sinvG Σ Γ α β τ, !MapAGΓ Γ, !MapMGΓ Γ, !memGΓ Γ}.
-  Context (n : level).
 
-  Lemma wctxr gi (SpcMap : univ_id → string → option fspec) (SpcMem : string → option fspec)
-      (MapInSpcMap : ∀ υ, spc_incl (MapAS.Spc υ n) (SpcMap υ)) :
-    w_ctx_refines
-      ((λ υ, (MapA.t υ n gi (SpcMap υ)) ★ (MemA.t gi SpcMem)), (MapA.InitCond ∗ MapM.InitCond)%I)
-      ((λ _, (MapI.t)                   ★ (MemA.t gi SpcMem)), emp%I).
+  Lemma wctxr
+      (u_s u_mem : univ_id)
+      (spc_s spc_mem : string → option fspec)
+      (LE : u_s >= 2)
+      (MapInSpcMap : spc_incl (MapAS.spc u_s) spc_s) :
+    ctx_refines
+      ((MapA.t u_s spc_s) ★ (MemA.t u_mem spc_mem), (MapA.init_cond ∗ MapM.init_cond)%I)
+      ((MapI.t)           ★ (MemA.t u_mem spc_mem), emp%I).
   Proof.
     etrans; cycle 1.
     { eapply MapIM.wctxr.
-      instantiate (1:= λ u, to_spc (MapMS.Spc u%positive n)).
-      i. split; try refl. unfold MapMS.Spc. unseal CRIS. prove_nodup.
+      instantiate (1:= to_spc (MapMS.spc 1)).
+      i. split; try refl. unfold MapMS.spc. unseal CRIS. prove_nodup.
     }
-    eapply w_ctx_refines_frameR.
-    eapply w_ctx_refines_cond_strengthen; first (instantiate (1:=(emp ∗ MapM.InitCond)%I)).
-    { iIntros "[_ $]". }
-    eapply w_ctx_refines_cond_frameR, MapMA.wctxr; eauto.
-    split; try refl.
-    rewrite /MapMS.Spc; unseal CRIS; prove_nodup.
+    eapply ctxr_frameR. rewrite -(hmod_addc_empty_l (MapM.t _ _)). eapply ctxr_cond_frameR.
+    eapply MapMA.wctxr; eauto. rewrite /MapMS.spc; unseal CRIS; prove_nodup. ss.
   Qed.
 End MapIA. End MapIA.
